Tests/Shards/Targets.lean
@@ -22,6 +22,7 @@ import Tests.Materialization.EngineeringDiskClosureV1
 import Tests.Materialization.Targets
 import Tests.Materialization.AleoPfAssetsV1
 import Tests.Materialization.NearHostModel
+import Tests.Materialization.NearStaticAlignmentV1
 import Tests.Materialization.NoirRelationModel
 import Tests.Materialization.NoirCompileAcceptance
 import Tests.Materialization.NoirAcirV1
@@ -100,6 +101,7 @@ unsafe def main : IO Unit := do
   Tests.Materialization.NoirAcirV1.run
   IO.eprintln "CP run"
   Tests.Materialization.NearHostModel.run
+  Tests.Materialization.NearStaticAlignmentV1.run
   IO.eprintln "CP run"
   Tests.Materialization.NoirRelationModel.run
   IO.eprintln "CP run"
